SpinLockAll complete

examples/spinlock/SpinLockAll.v
@@ -5,215 +5,352 @@ Require Import SpinLockMainHeader SpinLockMainI SpinLockMainA SpinLockMainIAProo
 Require Import SchHeader SchI SchA SchIAproof.
 Require Import ElimRel SModCancel Cancellation.
 
-(* From iris Require Import frac_auth numbers. *)
+Ltac gen_eq a :=
+  match a with context [?t] =>
+    lazymatch t with
+    | eq_refl => fail
+    | _ =>
+      let T := type of t in
+      match (eval simpl in T) with
+      | _ = _ => generalize t
+      end
+    end
+  end.
+
+Ltac gen_prop a :=
+  match a with context [?t] =>
+    let T := type of t in
+    match (eval simpl in T) with
+    | Prop => generalize t
+    end
+  end.
+
+Ltac remove_eq_aux :=
+  let e := fresh "E" in
+  intros e;
+  match goal with
+  | H : @eq ?A ?b _ |- _ => replace H with (@eq_refl A b)
+  end; last apply UIP; clear e.
+
+Ltac remove_eq a := gen_eq a; remove_eq_aux.
+
+From iris Require Import csum.
+
+Module InitRes.
+  Definition nil : GRAs.nil.
+  Proof. intros i; inv i. Defined.
+
+  Definition singleton {A : DRA} (a : option A) : GRAs.singleton A.
+  Proof.
+    intros i γ. inv_fin i.
+    { destruct (decide (γ = base_γ)).
+      { destruct a as [a|].
+        { ss. exact (Some (Cinr a)). }
+        { ss. exact (Some (Cinl (Excl ()))). }
+      }
+      { exact None. }
+    }
+    { intros i. inv i. }
+  Defined.
+
+  Definition R_prf {Σ1 Σ2 : GRA} (i2 : gid Σ2) :
+    @eq cmra
+    (allocs.allocsUR positive (@GRA_lookup Σ2 i2))
+    (allocs.allocsUR positive (@GRA_lookup (GRAs.app Σ1 Σ2) (Fin.R (@GRA_len Σ1) i2))).
+  Proof. rewrite /GRAs.app /= fin_add_inv_r; refl. Qed.
+
+  Definition L_prf {Σ1 Σ2 : GRA} (i1 : gid Σ1) :
+    @eq cmra
+    (allocs.allocsUR positive (@GRA_lookup Σ1 i1))
+    (allocs.allocsUR positive (@GRA_lookup (GRAs.app Σ1 Σ2) (Fin.L (@GRA_len Σ2) i1))).
+  Proof. rewrite /GRAs.app /= fin_add_inv_l; refl. Qed.
+
+  Definition R {Σ1 Σ2 : GRA} (r2 : Σ2) : GRAs.app Σ1 Σ2.
+  Proof.
+    intros i. eapply fin_add_inv with (i:=i).
+    { intros i1 g. exact ε. }
+    { intros i2. refine (cmra_transport (R_prf i2) (r2 i2)). }
+  Defined.
+
+  Definition L {Σ1 Σ2 : GRA} (r1 : Σ1) : GRAs.app Σ1 Σ2.
+  Proof.
+    intros i. eapply fin_add_inv with (i:=i).
+    { intros i1. refine (cmra_transport (L_prf i1) (r1 i1)). }
+    { intros i2 g. exact ε. }
+  Defined.
+
+  Lemma R_distr {Σ1 Σ2 : GRA} (r1 r2 : Σ2) : @R Σ1 Σ2 (r1 ⋅ r2) = @R Σ1 Σ2 r1 ⋅ @R Σ1 Σ2 r2.
+  Proof.
+    extensionalities i; apply fin_add_inv with (i:=i); clear i.
+    { intros i1; rewrite /R ?discrete_fun_lookup_op ?fin_add_inv_l //. }
+    { intros i2. rewrite /R discrete_fun_lookup_op fin_add_inv_r.
+      rewrite !fin_add_inv_r cmra_transport_op //.
+    }
+  Qed.
+
+  Lemma L_distr {Σ1 Σ2 : GRA} (r1 r2 : Σ1) : @L Σ1 Σ2 (r1 ⋅ r2) = @L Σ1 Σ2 r1 ⋅ @L Σ1 Σ2 r2.
+  Proof.
+    extensionalities i; apply fin_add_inv with (i:=i); clear i.
+    { intros i1. rewrite /L discrete_fun_lookup_op fin_add_inv_l.
+      rewrite !fin_add_inv_l cmra_transport_op //.
+    }
+    { intros i2; rewrite /L ?discrete_fun_lookup_op ?fin_add_inv_r //. }
+  Qed.
+
+  Definition app {Σ1 Σ2 : GRA} (r1 : Σ1) (r2 : Σ2) : GRAs.app Σ1 Σ2 :=
+    @L Σ1 Σ2 r1 ⋅ @R Σ1 Σ2 r2.
+
+  Lemma singleton_some_valid {A : DRA} (a : A)
+      (VALID : ✓ a) :
+    ✓ (singleton (Some a) ⋅ initial_resource_own_admin).
+  Proof.
+    intros i γ. inv_fin i; ss; des_ifs.
+    { rewrite ?discrete_fun_lookup_op /singleton /initial_resource_own_admin.
+      des_ifs. ss. rewrite left_id /allocs.allocs_auth; des_ifs; ss.
+    }
+    { intros i; inv i. }
+  Qed.
+
+  Lemma singleton_none_valid {A : DRA} :
+    ✓ (@singleton A None ⋅ initial_resource_own_admin).
+  Proof.
+    intros i γ. inv_fin i; ss; des_ifs.
+    { rewrite ?discrete_fun_lookup_op /singleton /initial_resource_own_admin.
+      des_ifs; ss; rewrite left_id /allocs.allocs_auth; des_ifs.
+    }
+    { intros i; inv i. }
+  Qed.
+
+  Definition app_valid {Σ1 Σ2 : GRA} (r1 : Σ1) (r2 : Σ2)
+      (VALID1 : ✓ (r1 ⋅ initial_resource_own_admin))
+      (VALID2 : ✓ (r2 ⋅ initial_resource_own_admin)) :
+    ✓ (app r1 r2 ⋅ initial_resource_own_admin).
+  Proof.
+    intros i; apply fin_add_inv with (i:=i).
+    { intros i1. rewrite /app ?discrete_fun_lookup_op.
+      rewrite /L fin_add_inv_l /R fin_add_inv_l right_id.
+      rewrite /initial_resource_own_admin.
+      match goal with | |- ?A => gen_eq A end.
+      rewrite /GRAs.app /= fin_add_inv_l. remove_eq_aux. ss.
+    }
+    { intros i2. rewrite /app ?discrete_fun_lookup_op.
+      rewrite /L fin_add_inv_r /R fin_add_inv_r left_id.
+      rewrite /initial_resource_own_admin.
+      match goal with | |- ?A => gen_eq A end.
+      rewrite /GRAs.app /= fin_add_inv_r. remove_eq_aux. ss.
+    }
+  Qed.
+
+  Lemma singleton_index {A : DRA} (a : A) :
+    singleton (Some a) = discrete_fun_singleton 0%fin (allocs.allocs_frag base_γ a).
+  Proof.
+    extensionalities i g. inv_fin i; ss; des_ifs.
+    { rewrite ?discrete_fun_lookup_singleton //=. }
+    { rewrite discrete_fun_lookup_singleton /= /allocs.allocs_frag discrete_fun_lookup_singleton_ne //. }
+    { intros i; inv i. }
+  Qed.
+
+  Lemma L_index {Σ1 Σ2 : GRA} (i : fin (@GRA_len Σ1)) r :
+    @L Σ1 Σ2 (discrete_fun_singleton i r)
+    = discrete_fun_singleton (Fin.L (@GRA_len Σ2) i) (cmra_transport (@L_prf Σ1 Σ2 i) r).
+  Proof.
+    rewrite /L. extensionalities i1.
+    apply fin_add_inv with (i:=i1); cycle 1.
+    { intros i2; ss.
+      match goal with | |- fin_add_inv ?P ?H1 ?H2 ?r = _ => rewrite (fin_add_inv_r P H1 H2 _) end.
+      rewrite discrete_fun_lookup_singleton_ne; ss.
+      ii. eapply Fin.L_R_neq; eauto.
+    }
+    { intros i2; ss.
+      destruct (decide (i = i2)).
+      { subst.
+        match goal with | |- fin_add_inv ?P ?H1 ?H2 ?r = _ => rewrite (fin_add_inv_l P H1 H2 _) end.
+        rewrite ?discrete_fun_lookup_singleton //.
+      }
+      { match goal with | |- fin_add_inv ?P ?H1 ?H2 ?r = _ => rewrite (fin_add_inv_l P H1 H2 _) end.
+        rewrite ?discrete_fun_lookup_singleton_ne //.
+        { match goal with | |- ?a => gen_eq a end.
+          rewrite /GRAs.app /= fin_add_inv_l. remove_eq_aux. ss.
+        }
+        { ii. apply Fin.L_inj in H. ss. }
+      }
+    }
+  Qed.
+
+  Lemma R_index {Σ1 Σ2 : GRA} (i : fin (@GRA_len Σ2)) r :
+    @R Σ1 Σ2 (discrete_fun_singleton i r)
+    = discrete_fun_singleton (Fin.R (@GRA_len Σ1) i) (cmra_transport (@R_prf Σ1 Σ2 i) r).
+  Proof.
+    rewrite /R. extensionalities i1.
+    apply fin_add_inv with (i:=i1); cycle 1.
+    { intros i2; ss.
+      match goal with | |- fin_add_inv ?P ?H1 ?H2 ?r = _ => rewrite (fin_add_inv_r P H1 H2 _) end.
+      destruct (decide (i = i2)).
+      { subst. rewrite ?discrete_fun_lookup_singleton //.
+      }
+      { rewrite ?discrete_fun_lookup_singleton_ne //.
+        { match goal with | |- ?a => gen_eq a end.
+          rewrite /GRAs.app /= fin_add_inv_r. remove_eq_aux. ss.
+        }
+        { ii. apply Fin.R_inj in H. ss. }
+      }
+    }
+    { intros i2; ss.
+      match goal with | |- fin_add_inv ?P ?H1 ?H2 ?r = _ => rewrite (fin_add_inv_l P H1 H2 _) end.
+      rewrite discrete_fun_lookup_singleton_ne; ss.
+      ii. eapply Fin.L_R_neq; eauto.
+    }
+  Qed.
+End InitRes.
+Notation "*[ ]" := InitRes.nil (format "*[ ]").
+Notation "*[ Σ1 ; .. ; Σn ]" :=
+  (InitRes.app (InitRes.singleton Σ1) .. (InitRes.app (InitRes.singleton Σn) InitRes.nil) ..).
+Notation "**[ Σ1 ; .. ; Σn ]" := (InitRes.app Σ1 .. (InitRes.app Σn InitRes.nil) ..).
+
+Ltac unfold_own :=
+  match goal with
+  | |- Own ?R = own base_γ ?R2 =>
+    rewrite own.Own_eq /own.Own_def own.own_eq /own.own_def /own.iRes_singleton; f_equal
+  end.
+
+Ltac unfold_left :=
+  repeat match goal with
+  | |- context [InitRes.singleton _] => rewrite InitRes.singleton_index
+  | |- context [InitRes.L (discrete_fun_singleton _ _)] => rewrite ?InitRes.L_index
+  | |- context [InitRes.R (discrete_fun_singleton _ _)] => rewrite ?InitRes.R_index
+  end.
+
+Hint Unfold invG_I invG_Σ invG_subG subG_invΣ subG_inG : GRA_index.
+Hint Unfold sProp.in_subG_obligation_1 in_subG invG_E invG_Γ subG_invΓ invG_D : GRA_index.
+
+Ltac solve_index H := 
+  eapply eq_ind; first iExact H;
+  unfold_own;
+  etrans;
+  [unfold_left; repeat match goal with | |- ?a = _ => remove_eq a end; simpl; refl
+  | etrans; cycle 1;
+    [ symmetry;
+      let k := fresh "k" in
+      match goal with
+      | |- context [inG_id ?i] => pattern i; match goal with | |- ?f ?a => set (k:=f) end
+      end;
+      autounfold with GRA_index
+      ; subst k
+      ; simpl
+      ; hrepeat do 1 match goal with | |- ?a = _ => remove_eq a end
+      ; simpl
+    | refl
+    ]
+  ].
+
+Lemma ir_own_admin {Σ : GRA} : Own initial_resource_own_admin ⊢ own_admin.
+Proof.
+  rewrite own.own_admin_eq /own.own_admin_def.
+  iIntros "H". iExists (⊤ ∖ {[base_γ]}).
+  iSplit.
+  { iPureIntro. eapply difference_infinite, singleton_finite. eapply top_infinite. }
+  { rewrite /initial_resource_own_admin own.Own_eq /own.Own_def. iFrame. }
+Qed.
+
 Module SpinLockAll.
-  Local Existing Instances invG_Σ invG_Γ invG_I invG_E invG_D.
-
-  Instance τ : TypG.t := λ _, ST.t.
-  Instance typG : CtxST.t τ. Proof. econs. econs. instantiate (1:=0); ss. Qed.
-
-  Local Instance Γ : HRA := ##[invΓ; memΓ; SchAΓ; SpinLockΓ; SpinLockMainAΓ].
-  Local Instance α : SRFCons.t :=
-    λ n,
-      match n with
-      | 0 => SL.syntax
-      | _ => inv_syntax
-      end.
-  Local Instance Σ : GRA := ##[invΣ; SchAΣ; Γ].
-  Local Instance sub : subG Γ Σ.
-  Proof. do 2 apply subG_app_r. apply subG_refl. Defined.
-  Local Instance invG : invG α Σ Γ.
-  Proof. econs. { econs. exists 0%fin. ss. } { econs. { exists 0%fin. ss. } { exists 1%fin. ss. } } Defined.
-  Instance β : SRFIntp.t :=
-    λ n,
-      match n with
-      | 0 => SL.interp
-      | _ => inv_interp
-      end.
-  Local Instance intpG : SRFIntp.inG (@SL.syntax τ Γ) α (@SL.interp τ α Γ Σ _) β.
-  Proof. econs; instantiate (1:=0); ss. Qed.
-
-  Local Instance invintpG : SRFIntp.inG inv_syntax α inv_interp β.
-  Proof. econs; instantiate (1:=1); ss. Qed.
-
-  Local Instance sinvg : sinvG Σ Γ α β τ.
-  Proof. econs; econs; try typeclasses eauto. Qed.
-
-  Local Instance memΓ : memGΓ Γ.
-  Proof. econs. exists 2%fin; ss. Defined.
-
-  Local Instance SchAΓ : SchAGΓ Γ.
-  Proof. econs. exists 3%fin; ss. Defined.
-
-  Local Instance SpinLockAGΓ : SpinLockAGΓ Γ.
-  Proof. econs. exists 4%fin; ss. Defined.
-
-  Local Instance SpinLockMainAGΓ : SpinLockMainAGΓ Γ.
-  Proof. econs. exists 5%fin; ss. Defined.
-
-  Local Instance SchAΣ : SchAGΣ Σ.
-  Proof. econs. exists 1%fin; ss. Defined.
-
-  (* building the target module *)
-  Local Definition csl : string → bool := λ _, false.
-  Local Definition genv : GEnv.t := GEnv.unit.
-  Local Definition mod_tgt : HMod.t := SpinLockMainI.t ★ MemI.t csl genv ★ SchI.t ★ SpinLockI.t.
-
-  (* building the source module *)
-  Local Definition u : univ_id := 1.
-
-  Local Definition spc_user_s : string → option fspec :=
-    to_spc (SpinLockMainAS.spc u ++ MemA.Spc ++ SpinLockAS.spc u).
-
-  Local Definition smod_src : SMod.t :=
-    SpinLockMainA.Mod u ☆ MemA.Mod ☆ SchA.Mod u spc_user_s ☆ SpinLockA.Mod u.
-  Local Definition spc_s : string → option fspec :=
-    spc_from smod_src.
-  Local Definition mod_src : HMod.t := SMod.to_hmod (wsim_ginv u ⊤) spc_s smod_src.
-  Local Definition init_cond : iProp Σ := (MemA.InitCond csl genv ∗ SchA.InitCond)%I.
-
-  (* source module after cancellation *)
-  Local Definition smod_cancel : HMod.t := SModCancel.to_hmod smod_src.
-
-  (* Refinement between smod_cancel and smod_src *)
-  Local Definition main_fsp : fspec := SpinLockMainAS.main_spec u.
-  Lemma cancel_src :
-    refines (smod_cancel, init_cond ∗ main_fsp.(precond) tt tt↑ tt↑)%I
-            (mod_src,     init_cond).
-  Proof. eapply cancellation; try by econs. i. unfold_pre_post. iIntros "[_ [-> ->]]". done. Qed.
-
-  (* Refinement between smod_src and mod_tgt *)
-  Lemma src_tgt : refines (mod_src, init_cond) (mod_tgt, emp%I).
-  Proof.
-    apply ctxr_refines.
-    rewrite /mod_src /smod_src /mod_tgt /init_cond ?add_interp_comm.
-    replace (SMod.to_hmod _ _ (SpinLockMainA.Mod _)) with (SpinLockMainA.t u spc_s); cycle 1.
-    { unfold_hmod; ss. }
-    replace (SMod.to_hmod _ _ (MemA.Mod)) with (MemA.t u spc_s); cycle 1.
-    { unfold_hmod; ss. }
-    replace (SMod.to_hmod _ _ (SpinLockA.Mod _)) with (SpinLockA.t u spc_s); cycle 1.
-    { unfold_hmod; ss. }
-
-    etrans.
-    { do 2 eapply ctxr_frameL. eapply ctxr_comm. }
-    do 2 rewrite -hmod_add_assoc.
-    etrans.
-    { eapply ctxr_frameR.
-      rewrite hmod_add_assoc -hmod_addc_empty_l.
-      etrans; first eapply ctxr_cond_frameR.
-      { eapply SpinLockMainIA.wctxr; eauto.
-        { instantiate (1:=spc_user_s).
-          rewrite /spc_user_s /SchAS.spc /spc_s /smod_src; unseal CRIS. split; first prove_nodup.
-          ii. ss; des_ifs; rewrite ->eq_rel_dec_correct in *; des_ifs.
-        }
-        { rewrite /spc_user_s /SchAS.spc /spc_s /smod_src; unseal CRIS. split; first prove_nodup.
-          ii. ss; des_ifs; rewrite ->eq_rel_dec_correct in *; des_ifs.
-        }
-        { rewrite /spc_user_s /MemA.Spc /spc_s /smod_src; unseal CRIS. split; first prove_nodup.
-          ii. ss; des_ifs; rewrite ->eq_rel_dec_correct in *; des_ifs.
-        }
-      }
-      rewrite hmod_addc_empty_l. refl.
-    }
-    rewrite hmod_add_assoc. eapply ctxr_frameL.
-    etrans.
-    { eapply ctxr_frameR. rewrite -hmod_addc_empty_l. eapply ctxr_cond_frameR.
-      etrans; first eapply ctxr_comm.
-      eapply SpinLockIA.wctxr.
-      { rewrite /spc_user_s /SchAS.spc /spc_s /smod_src; unseal CRIS. split; first prove_nodup.
-        ii. ss; des_ifs; rewrite ->eq_rel_dec_correct in *; des_ifs.
-      }
-      { rewrite /spc_user_s /spc_s /smod_src /MemA.Spc; unseal CRIS. split; first prove_nodup.
-        ii. ss; des_ifs; rewrite ->eq_rel_dec_correct in *; des_ifs.
-      }
-    }
-    rewrite hmod_add_assoc.
-    etrans; first eapply ctxr_comm. rewrite -hmod_add_assoc. eapply ctxr_frameR.
-    etrans.
-    { rewrite hmod_addc_empty_l. eapply ctxr_frameR, ctxr_cond_frameR. eapply MemIA.wctxr.
-      rewrite /MemA.Spc; unseal CRIS.
-      split; first prove_nodup. ii; ss; des_ifs; rewrite ->eq_rel_dec_correct in *; des_ifs.
-    }
-    eapply ctxr_frameL.
-    etrans.
-    { replace (SMod.to_hmod _ _ (SchA.Mod _ _)) with (SchA.t u spc_s spc_user_s); cycle 1.
-      { unfold_hmod; ss. }
-      rewrite hmod_addc_empty_l.
-      eapply SchIA.wctxr.
-      { rewrite /spc_user_s /SchAS.spc /spc_s /smod_src; unseal CRIS. split; first prove_nodup.
-        ii. ss; des_ifs; rewrite ->eq_rel_dec_correct in *; des_ifs.
-      }
-      { rewrite /spc_user_s /SchAS.spc /spc_s /smod_src /MemA.Spc; unseal CRIS.
-        ii. ss; des_ifs; rewrite ->eq_rel_dec_correct in *; des_ifs.
-      }
-    }
-    refl.
-  Qed.
-
-  Lemma cancel_tgt :
-    refines (smod_cancel, (init_cond ∗ (main_fsp).(precond) tt tt↑ tt↑)%I)
-            (mod_tgt, emp%I).
-  Proof.
-    etrans.
-    { eapply cancel_src. }
-    { eapply src_tgt. }
-  Qed.
-
-  Import rListNotations.
-  Local Definition initial_resource_list : res_list :=
-    [ownIRA_resource u; ownERA_resource u; ownDRA_resource u;
-     SchAS.tidRA_resource; SchAS.threadsRA_resource; memRA_resource csl genv]%res_list.
-
-  Local Definition initial_resource : Σ := 
-    (op_res_list initial_resource_list) ⋅ initial_resource_own_admin.
-
-  Ltac dfs_solve :=
-    econs; [repeat (intros [C | C]; [inv C|]; revert C); intros []|].
-    
-  Lemma initial_resource_valid : ✓ initial_resource.
-  Proof.
-    apply op_res_list_valid.
-    repeat dfs_solve. econs.
-  Qed.
-
-  Theorem behavioral_refinement :
-    ∃ target_resource, refines_mod
-      (HMod.to_mod smod_cancel initial_resource)
-      (HMod.to_mod mod_tgt target_resource).
-  Proof.
-    move: (cancel_tgt)=>H; rewrite /refines in H; ss.
-    destruct (H initial_resource).
-    { apply initial_resource_valid. }
-    { iIntros "H". iPoseProof (big_bang with "H") as "[O H]".
-      iDestruct "H" as "[H1 [H2 [H3 [H4 [H5 [H6 _]]]]]]"; iFrame.
-      iPoseProof (ownI_initial_gen with "[$]") as "[U W]".
-      iPoseProof (SchAS.tid_admin_none_split with "[H4]") as "[H3 H4]".
-      { rewrite /SchAS.tid_admin; unseal "SchA"; ss. }
-      iFrame. des_ifs. unfold_pre_post. iSplitL.
-      { iSplitR "H5".
-        { iDestruct "H6" as "[$ $]". }
-        { rewrite /SchAS.initial_threads. unseal "SchA". done. }
-      }
-      iSplit; eauto.
-    }
-    { econs; ss; prove_nodup. }
-    { exists x; des; eauto. }
-  Qed.
-End SpinLockAll.
-
-Module SpinLockAllFail.
   Import inv_instances.
-  Local Instance Γ : HRA := ##[invΓ; memΓ; SchAΓ; SpinLockΓ; SpinLockMainAΓ].
-  Local Instance Σ : GRA := ##[invΣ; SchAΣ; Γ].
+  Local Definition u : univ_id := 1.
 
-  (* building the target module *)
   Local Definition csl : string → bool := λ _, false.
   Local Definition genv : GEnv.t := GEnv.unit.
+
+  Local Instance Γ : HRA := ##[invΓ; memΓ; SchAΓ; SpinLockΓ; SpinLockMainAΓ].
+
+  Definition IRownIRA : DRA_mk ownIRA :=
+    ownI_initial u.
+  Lemma IRownIRA_valid : ✓ (IRownIRA). eapply (ownI_initial_valid u). Qed.
+
+  Local Instance Σ : GRA := ##[invΣ; SchAΣ; Γ].
+
+  Definition IRownDRA : DRA_mk ownDRA :=
+    ownD_initial u.
+  Lemma IRownDRA_valid : ✓ (IRownDRA). eapply ownD_initial_valid. Qed.
+
+  Definition IRownERA : DRA_mk ownERA :=
+    ownE_initial u.
+  Lemma IRownERA_valid : ✓ (IRownERA). eapply ownE_initial_valid. Qed.
+
+  Definition IRmemRA : DRA_mk memRA :=
+    mem_initial_mem_r csl genv.
+  Lemma IRmemRA_valid : ✓ (IRmemRA).
+  Proof. pose proof (mem_initial_valid csl genv). rewrite /IRmemRA. eapply cmra_valid_op_l; eauto. Qed.
+
+  Definition IRthreadsRA : DRA_mk threadsRA :=
+    SchAS.threadsRA_initial.
+  Lemma IRthreadsRA_valid : ✓ (IRthreadsRA). apply SchAS.threadsRA_initial_valid. Qed.
+
+  Definition IRtidRA : DRA_mk tidRA :=
+    SchAS.tidRA_initial.
+  Lemma IRtidRA_valid : ✓ (IRtidRA). apply SchAS.tidRA_initial_valid. Qed.
+
+  Definition IRinvΓ : invΓ :=
+    *[Some (IRownERA); Some (IRownDRA)].
+  Definition IRmemΓ : memΓ :=
+    *[Some IRmemRA].
+  Definition IRSchAΓ : SchAΓ :=
+    *[Some IRtidRA].
+
+  Definition IRΓ : Γ :=
+    **[IRinvΓ; IRmemΓ; IRSchAΓ; *[None]; *[None]].
+
+  Definition IRΣ : Σ :=
+    **[*[Some (IRownIRA)]; *[Some IRthreadsRA]; IRΓ].
+
+  Lemma IRΣ_valid : ✓ (IRΣ ⋅ initial_resource_own_admin).
+  Proof.
+    eapply InitRes.app_valid.
+    { apply InitRes.app_valid.
+      { apply InitRes.singleton_some_valid, IRownIRA_valid. }
+      { intros i; inv_fin i. }
+    }
+    apply InitRes.app_valid.
+    { apply InitRes.app_valid.
+      { apply InitRes.singleton_some_valid, IRthreadsRA_valid. }
+      { intros i; inv_fin i. }
+    }
+    apply InitRes.app_valid.
+    { apply InitRes.app_valid.
+      { apply InitRes.app_valid.
+        { apply InitRes.singleton_some_valid, IRownERA_valid. }
+        { apply InitRes.app_valid.
+          { apply InitRes.singleton_some_valid, IRownDRA_valid. }
+          { intros i; inv_fin i. }
+        }
+      }
+      apply InitRes.app_valid.
+      { apply InitRes.app_valid.
+        { apply InitRes.singleton_some_valid, IRmemRA_valid. }
+        { intros i; inv_fin i. }
+      }
+      apply InitRes.app_valid.
+      { apply InitRes.app_valid.
+        { apply InitRes.singleton_some_valid, IRtidRA_valid. }
+        { intros i; inv_fin i. }
+      }
+      apply InitRes.app_valid.
+      { apply InitRes.app_valid.
+        { apply InitRes.singleton_none_valid. }
+        { intros i; inv_fin i. }
+      }
+      apply InitRes.app_valid.
+      { apply InitRes.app_valid.
+        { apply InitRes.singleton_none_valid. }
+        { intros i; inv_fin i. }
+      }
+      { intros i; inv_fin i. }
+    }
+    { intros i; inv_fin i. }
+  Qed.
+
+  (* building the target module *)
   Local Definition mod_tgt : HMod.t := SpinLockMainI.t ★ MemI.t csl genv ★ SchI.t ★ SpinLockI.t.
 
   (* building the source module *)
-  Local Definition u : univ_id := 1.
-
   Local Definition spc_user_s : string → option fspec :=
     to_spc (SpinLockMainAS.spc u ++ MemA.Spc ++ SpinLockAS.spc u).
 
@@ -223,6 +360,7 @@ Module SpinLockAllFail.
     spc_from smod_src.
   Local Definition mod_src : HMod.t := SMod.to_hmod (wsim_ginv u ⊤) spc_s smod_src.
   Local Definition init_cond : iProp Σ := (MemA.InitCond csl genv ∗ SchA.InitCond)%I.
+  Definition a : invG α Σ Γ. apply _. Defined.
 
   (* source module after cancellation *)
   Local Definition smod_cancel : HMod.t := SModCancel.to_hmod smod_src.
@@ -310,65 +448,44 @@ Module SpinLockAllFail.
     { eapply src_tgt. }
   Qed.
 
-  Import rListNotations.
-  Local Definition initial_resource_list : res_list :=
-    [ownIRA_resource u; ownERA_resource u; ownDRA_resource u; SchAS.tidRA_resource; SchAS.threadsRA_resource]%res_list.
-  Local Definition initial_resource : Σ := 
-    (op_res_list initial_resource_list) ⋅ initial_resource_own_admin.
+  Notation "'L'" := InitRes.L (at level 50, only printing).
+  Notation "'R'" := InitRes.R (at level 50, only printing).
 
-  Ltac solve_eq_index :=
-    match goal with
-    | H : eq_index ?r ?r2 |- _ => revert H; autounfold with GRA_index; intros H; rewrite /eq_index in H
-    end; des_ifs;
-    match goal with
-    | H1 : @eq (inG _ _) ?a _, H2 : @eq (inG _ _) ?b _ |- _ =>
-        let H := fresh "H" in assert (H : inG_id a = inG_id b) by rewrite H1 H2 //=;
-        repeat match goal with
-        | H : inG_id ?a = inG_id ?b |- _ => rewrite /a /b in H
-        end;
-        (* rewrite /a /b in H *)
-        revert H; autounfold with GRA_index; inv_instances.solve_in_subG_goal;
-        rewrite /eq_rec_r /eq_rec /= /subG_inG -!eq_rect_eq //=
-    end.
-  Ltac solve_nin_aux :=
-    match goal with
-    | H : r_In ?RES (r_cons ?RA ?RES' ?tl) |- _ => destruct H as [EQ | IN]; [solve_eq_index| solve_nin_aux]
-    | H : r_In ?RES (r_nil) |- _ => inv H
-    end.
-  Ltac solve_nin := ii; solve_nin_aux.
-  Ltac dfs_solve :=
-    match goal with
-    | |- r_NoDup (r_cons ?RA ?RES ?tl) => econs; [solve_nin|dfs_solve]
-    | |- r_NoDup (r_nil) => econs
-    end.
-  Hint Unfold sProp.in_subG_obligation_1 in_subG subG_invΣ subG_invΓ invG_subG invΓ invΣ invG_Σ invG_Γ invG_D invG_E invG_I SchAΣ : GRA_index.
-  Hint Unfold ownIRA_resource ownERA_resource ownDRA_resource SchAS.tidRA_resource SchAS.threadsRA_resource : GRA_index.
+  Hint Unfold SchA.RA_inG SchA.RA_inG0 SchA.subG_GΣ SchA.subG_GΓ : GRA_index.
 
   Theorem behavioral_refinement :
     ∃ target_resource, refines_mod
-      (HMod.to_mod smod_cancel initial_resource)
+      (HMod.to_mod smod_cancel (IRΣ ⋅ initial_resource_own_admin))
       (HMod.to_mod mod_tgt target_resource).
   Proof.
     move: (cancel_tgt)=>H; rewrite /refines in H; ss.
-    destruct (H initial_resource).
-    { apply op_res_list_valid. rewrite /initial_resource_list. dfs_solve. }
-    { iIntros "H". iPoseProof (big_bang with "H") as "[O H]".
-      iPoseProof (ownI_initial_gen with "[H]") as "[U W]".
-      { rewrite /initial_resource_list; s. des_ifs. rename inG_id into i.
-        assert (H' : inG_id invariants.ownIRA_resource_obligation_1 = i).
-        { rewrite Heq; ss. }
-        revert H'. rewrite /invariants.ownIRA_resource_obligation_1 /invG_I. autounfold with GRA_index.
-        rewrite inG_id_subG_inG subG_app_l_inG_id /eq_rec_r /eq_rec -eq_rect_eq.
-        intros H'; ss.
-        iDestruct "H" as "[H1 [H2 [H3 _]]]"; iFrame.
-        eapply eq_ind; first iExact "H1".
-        f_equiv. ss.
+    destruct (H ((IRΣ ⋅ initial_resource_own_admin))).
+    { apply IRΣ_valid. }
+    { rewrite /IRΣ /InitRes.app.
+      try (repeat rewrite ?InitRes.L_distr ?InitRes.R_distr).
+      iIntros "[[[I _] [[THS _] [[[E [D _]] [[M _] [[TID _] _]]] _]]] O]".
+      iPoseProof (ownI_initial_gen u with "[I E D]") as "[U W]".
+      { iSplitL "I".
+        { solve_index "I". f_equal. }
+        iSplitL "E".
+        { solve_index "E". f_equal. }
+        { solve_index "D". f_equal. }
       }
-      iFrame. unfold_pre_post. iSplitL.
-      { rewrite /init_cond. admit. }
-      admit.
+      iAssert (SchAS.tid_admin None) with "[TID]" as "TID".
+      { rewrite /SchAS.tid_admin. unseal "SchA". solve_index "TID". f_equal. }
+      iPoseProof (SchAS.tid_admin_none_split 0 with "TID") as "[H1 H2]".
+      { iSplitR "U W O H2"; cycle 1.
+        { iPoseProof (ir_own_admin with "O") as "$". unfold_pre_post; iFrame. iSplit; eauto. }
+        rewrite /init_cond. iSplitL "M".
+        { rewrite /MemA.InitCond /mem_initial_mem. solve_index "M". f_equal. }
+        iSplitL "THS".
+        { rewrite /SchAS.initial_threads. unseal "SchA". rewrite /IRthreadsRA /SchAS.threadsRA_initial.
+          solve_index "THS". f_equal.
+        }
+        { iFrame. }
+      }
     }
     { econs; ss; prove_nodup. }
     { exists x; des; eauto. }
-     
-  Admitted.
+  Qed.
+End SpinLockAll.
