theories/iris_system/ucmra_list.v
@@ -1,7 +1,238 @@
 (* list of ucmras. Exists to avoid universal inconsistency of Iris and list with relations.  *)
-From iris.algebra Require Import cmra.
+(* From iris.algebra Require Import cmra.
+Require Import iprop sflib.
 
-Inductive cmra_list : Type :=
+Declare Scope clist_scope.
+Delimit Scope clist_scope with clist.
+
+Module CmraList.
+  Definition elem : Type := {R : cmra & option R}.
+
+  Inductive t : Type :=
+  | nil : t
+  | cons (a : elem) (l : t) `{CmraDiscrete (projT1 a)} : t.
+  Bind Scope clist_scope with t.
+
+  Local Open Scope clist_scope.
+
+  Definition length : t → nat :=
+    fix length l :=
+      match l with
+      | nil => O
+      | cons _ l' => S (length l')
+      end.
+
+  Definition app : t → t → t :=
+    fix app l m :=
+      match l with
+      | nil => m
+      | cons a l1 => cons a (app l1 m)
+      end.
+
+  Fixpoint In (a : elem) (l : t) : Prop :=
+    match l with
+    | nil => False
+    | cons hd tl => a = hd ∨ In a tl
+    end.
+
+  Definition incl (l1 l2 : t) : Prop := ∀ a, In a l1 → In a l2.
+
+  Lemma incl_tl (a : elem) (l1 l2 : t) `{CmraDiscrete (projT1 a)} :
+    incl l1 l2 → incl l1 (cons a l2).
+  Proof. intros INCL i IN1; ss; right; apply INCL; eauto. Qed.
+
+  Lemma incl_cons (a : elem) (l1 l2 : t) `{CmraDiscrete (projT1 a)} :
+    In a l2 → incl l1 l2 → incl (cons a l1) l2.
+  Proof. intros IN INCL; intros i [IN1 | IN1]; subst; eauto. Qed.
+
+  Lemma incl_cons_inv (a : elem) (l1 l2 : t) `{CmraDiscrete (projT1 a)} :
+    incl (cons a l1) l2 → In a l2 ∧ incl l1 l2.
+  Proof. intros INCL; split; [eapply INCL; ss; eauto|intros i IN; eapply INCL; right; eauto]. Qed.
+
+  Definition to_GRA (l : t) : GRA.
+  Proof.
+    induction l as [|[R hd] tl].
+    { refine (GRA_mk 0 _). intros a; inv a. }
+    { refine (GRA_mk (1 + GRA_len) _). intros i; inv_fin i.
+      { apply (DRA_mk R). }
+      { apply IHtl. }
+    }
+  Defined.
+
+  (* Lemma app_to_GRA (l1 l2 : t) : to_GRA (app l1 l2) = GRAs.app (to_GRA l1) (to_GRA l2).
+  Proof.
+    induction l1.
+    { ss. destruct (to_GRA l2); ss. }
+  Admitted.
+
+  Class sub (l : t) (Σ : GRA) := sub_in i : In i l → { j | projT1 i = @GRA_lookup Σ j }.
+  Global Instance sub_refl l : sub l (to_GRA l).
+  Proof. Admitted.
+
+  Global Instance sub_app_l l l1 l2 : sub l (to_GRA l1) → sub l (to_GRA (app l1 l2)).
+  Proof. Admitted.
+
+  Global Instance sub_app_r l l1 l2 : sub l (to_GRA l2) → sub l (to_GRA (app l1 l2)).
+  Proof. Admitted. *)
+
+  Fixpoint In_cmra (a : cmra) (l : t) : Prop :=
+    match l with
+    | nil => False
+    | cons hd tl => a = projT1 hd ∨ In_cmra a tl
+    end.
+
+  Class InCL (A : cmra) (l : t) := InCL_in : In_cmra A l.
+  Global Instance InCL_cons A a l `{CmraDiscrete A} : InCL A (cons (existT A a) l).
+  Proof. ss; eauto. Qed.
+
+  Global Instance InCL_tl A B l `{CmraDiscrete (projT1 B)} : InCL A l → InCL A (cons B l).
+  Proof. ss; eauto. Qed.
+
+  (* Global Instance InCL_sub_inG a l Σ : InCL a l → sub l Σ → inG a Σ.
+  Proof. Admitted. *)
+End CmraList.
+Global Coercion CmraList.to_GRA : CmraList.t >-> GRA.
+Infix "::" := CmraList.cons (at level 60, right associativity) : clist_scope.
+Infix "++" := CmraList.app (right associativity, at level 60) : clist_scope.
+
+Module GRAL.
+  Inductive t : Type :=
+  | nil
+  | cons (l : CmraList.t) (tl : t).
+
+  Fixpoint to_GRA (l : t) :=
+    match l with
+    | nil => GRAs.nil
+    | cons l tl => GRAs.app l (to_GRA tl)
+    end.
+
+  Fixpoint In (e : CmraList.t) (l : t) :=
+    match l with
+    | nil => False
+    | cons hd tl => e = hd ∨ In e tl
+    end.
+
+  Class sub (e : CmraList.t) (l : t) := sub_in : In e l.
+
+  Global Instance sub_cons a l : sub a (cons a l).
+  Proof. ss; eauto. Qed.
+
+  Global Instance sub_tl a b l : sub a l → sub a (cons b l).
+  Proof. ss; eauto. Qed.
+
+  Global Instance InCL_sub_inG a e l : CmraList.InCL a e → sub e l → inG a (to_GRA l).
+  Proof.
+    revert a e; induction l.
+    { intros ??? []. }
+  Admitted.
+
+  Section test.
+    Context (a b c : CmraList.t).
+    Let l := cons a (cons b (cons c nil)).
+    Goal sub c l. apply _. Qed.
+  End test.
+
+  Section test.
+    Context (a b c d e f g h i : cmra) `{∀ c, CmraDiscrete c}.
+    Local Open Scope clist_scope.
+    Import SigTNotations.
+    Let A := (a; None) :: (b; None) :: (c; None) :: CmraList.nil.
+    Let B := (d; None) :: (e; None) :: (f; None) :: CmraList.nil.
+    Let C := (e; None) :: (f; None) :: (g; None) :: CmraList.nil.
+    Local Instance Σ : GRA := GRAL.to_GRA (GRAL.cons A (GRAL.cons B (GRAL.cons C GRAL.nil))).
+    Goal inG g Σ. apply _. Qed.
+  End test.
+
+  Section test.
+    Context (a b c : cmra) `{∀ c, CmraDiscrete c}.
+    Local Open Scope clist_scope.
+    Import SigTNotations.
+    Let A := (a; None) :: (b; None) :: (c; None) :: CmraList.nil.
+    Context `{GRAL.sub A Γ}.
+    Goal inG a (to_GRA Γ). apply _. Qed.
+  End test.
+
+  Definition init_res (l : t) : GRAUR (to_GRA l).
+  Proof.
+    induction l as [|hd tl].
+    { exact ε. }
+    { simpl. admit. }
+
+End GRAL.
+(** Standard notations for lists.
+In a special module to avoid conflicts. *)
+Notation "#[ ]" := CmraList.nil (format "#[ ]") : clist_scope.
+Notation "#[ x ; .. ; z ]" := 
+  (CmraList.cons x .. (CmraList.cons z CmraList.nil) ..)
+    (format "#[ '[' x ;  '/' .. ;  '/' z ']' ]") : clist_scope.
+
+Section test.
+  Context `{!CmraDiscrete A, !CmraDiscrete B, !CmraDiscrete C, c : C}.
+  Import SigTNotations.
+  Local Open Scope clist_scope.
+  Local Definition b : CmraList.t := #[(A; None); (B; None); (C; Some c)].
+  Goal CmraList.InCL A b. apply _. Qed.
+
+  Local Instance Σ : GRA := CmraList.nil ++ CmraList.nil ++ b.
+  Goal inG A Σ. apply _. Qed.
+End test.
+
+Require Import own.
+Definition to_res (l : CmraList.t) : l.
+Proof.
+  induction l as [|[R [r|]] tl].
+  { exact ε. }
+  { refine (own.iRes_singleton base_γ r ⋅ _).
+    { Set Printing All. refine (inG_mk R _ 0%fin). } }
+
+Local Open Scope clist_scope.
+Global Instance incl_subG (l1 l2 : CmraList.t) : CmraList.incl l1 l2 → subG l1 l2.
+Proof.
+  induction l1.
+  { intros _ i; inv i. }
+  { intros [IN INCL]%CmraList.incl_cons_inv. i. destruct a. simpl in i. inv_fin i.
+    { hexploit (INCL (existT x o)); first ss; eauto. admit. }
+    {  } }
+  intros H i; destruct (H i) as [j Hprf].
+  eexists. Set Printing All.  rewrite CmraList.to_GRA_len_app. rewrite Hprf. rewrite /CmraList.to_GRA /CmraList.t_rect. Set Printing All. reflexivity. *)
+
+
+(* Debug #1 *)
+(* From iris Require Import excl auth numbers.
+
+Class AGΣ (Σ : GRA) := {
+  #[local] A_inG :: inG (exclR unitO) Σ;
+}.
+Definition AΣ : GRA := #[DRA_mk (exclR unitO) None].
+Global Instance subG_AGΣ {Σ : GRA} : subG AΣ Σ → AGΣ Σ.
+Proof. solve_inG. Qed.
+
+Section a.
+  Context `{!AGΣ Σ}.
+  Definition a : inG (exclR unitO) Σ. Proof. apply _. Defined.
+End a.
+
+Class BGΣ (Σ : GRA) := {
+  #[local] B_inG :: inG (authUR (optionUR (exclR unitO))) Σ;
+}.
+Definition BΣ : GRA := #[DRA_mk (authUR (optionUR (exclR unitO))) (Some (● (Excl' ())))].
+Global Instance subG_BGΣ {Σ : GRA} : subG BΣ Σ → BGΣ Σ.
+Proof. solve_inG. Qed.
+
+Section b.
+  Context `{!BGΣ Σ}.
+  Definition b : inG (authUR (optionUR (exclR unitO))) Σ. Proof. apply _. Defined.
+End b.
+
+Class CGΣ (Σ : GRA) := {
+  #[local] C_inG :: inG (ZR) Σ;
+}.
+Definition CΣ : GRA := #[DRA_mk (ZR) (Some 1%Z)].
+Global Instance subG_CGΣ {Σ : GRA} : subG CΣ Σ → CGΣ Σ.
+Proof. solve_inG. Qed. *)
+
+
+(* Inductive cmra_list : Type :=
  | nil : cmra_list
  | cons (a : cmra) (l : cmra_list) `{CmraDiscrete a} : cmra_list.
 
@@ -11,9 +242,9 @@ Bind Scope ulist_scope with cmra_list.
 
 Infix "::" := cons (at level 60, right associativity) : ulist_scope.
 
-Local Open Scope ulist_scope.
+Local Open Scope ulist_scope. *)
 
-Module UList.
+(* Module UList.
   Definition length : cmra_list → nat :=
     fix length l :=
       match l with
@@ -67,4 +298,4 @@ Module UList.
     Qed.
 End Elts. End UList.
 
-Export UList.UListNotations.
+Export UList.UListNotations. *)
